src/Gates/GateRules.v
@@ -2,6 +2,7 @@ Require Import QuantumLib.Quantum.
 Require Export ZXCore.
 Require Export GateDefinitions.
 Require Export CoreRules.
+Require Export DiagramRules.
 
 Local Open Scope ZX_scope.
 
@@ -61,4 +62,127 @@ Proof.
   unfold Z_semantics, phase_shift.
   simpl.
   lma.
+Qed.
+
+Lemma cnot_involutive : _CNOT_R ⟷ _CNOT_ ∝ n_wire 2. 
+Proof.
+  rewrite <- compose_assoc.
+  rewrite (compose_assoc (— ↕ (X 1 2 0))).
+  rewrite <- (stack_compose_distr (Z 2 1 0) (Z 1 2 0) — —).
+  rewrite Z_spider_1_1_fusion.
+  cleanup_zx.
+  rewrite (X_wrap_over_top_left 1 1).
+  rewrite (X_wrap_over_top_right 1 1) at 1.
+  rewrite <- wire_to_n_wire.
+  rewrite <- (wire_removal_l —) at 1.
+  rewrite <- (wire_removal_l —) at 6.
+  rewrite 2 stack_compose_distr.
+  rewrite (stack_assoc_back — — (X 1 2 0)).
+  rewrite (stack_assoc_back — — (X 2 1 0)).
+  simpl_casts.
+  rewrite wire_to_n_wire at 3 4 6 7.
+  rewrite n_wire_stack.
+  rewrite (compose_assoc (— ↕ (⊂ ↕ —))).
+  rewrite wire_to_n_wire at 4.
+  rewrite (nwire_stack_compose_topleft (X 2 1 0) (Z 2 2 (0 + 0))).
+  rewrite <- (nwire_stack_compose_botleft (Z 2 2 (0 + 0)) (X 2 1 0)).
+  repeat rewrite <- compose_assoc.
+  rewrite (compose_assoc _ (n_wire 2 ↕ (X 2 1 0))).
+  rewrite <- (stack_compose_distr (n_wire 2) (n_wire (1 + 1)) (X 2 1 0) (X 1 2 0)).
+  rewrite X_spider_1_1_fusion.
+  rewrite Rplus_0_r.
+  simpl; cleanup_zx; simpl_casts.
+  rewrite (compose_assoc _ (— ↕ — ↕ X 2 2 _)).
+  rewrite stack_assoc.
+  simpl_casts.
+  rewrite <- (stack_compose_distr — — (— ↕ X 2 2 _)).
+  cleanup_zx.
+  rewrite wire_to_n_wire at 7.
+  rewrite <- X_wrap_over_top_left.
+  rewrite (stack_assoc_back — ⊂ —).
+  rewrite stack_assoc_back.
+  simpl_casts.
+  rewrite <- (stack_compose_distr (— ↕ ⊂) (Z 2 2 _ ↕ —) — —).
+  cleanup_zx.
+  rewrite wire_to_n_wire at 1.
+  rewrite <- (cast_id (eq_sym (Nat.add_0_r _)) (wrap_under_dimension 1) (n_wire 1 ↕ ⊂)).
+  rewrite <- Z_wrap_under_bot_left.
+  assert (1 = 1 + 0)%nat as Hcast by lia;
+  rewrite <- (cast_id Hcast (eq_refl) (Z _ (1 + 2) _));
+  simpl_casts;
+  clear Hcast.
+  rewrite wire_to_n_wire.
+  rewrite grow_Z_bot_right.
+  rewrite grow_X_top_left.
+  rewrite stack_nwire_distribute_r.
+  rewrite stack_nwire_distribute_l.
+  repeat rewrite <- compose_assoc.
+  rewrite (compose_assoc _ (n_wire 1 ↕ Z 1 2 0 ↕ n_wire 1)).
+  rewrite stack_assoc.
+  simpl_casts.
+  rewrite <- wire_to_n_wire.
+  rewrite <- (stack_compose_distr — — (Z 1 2 0 ↕ —)).
+  rewrite <- stack_compose_distr.
+  cleanup_zx.
+  rewrite hopf_rule_Z_X.
+  rewrite wire_to_n_wire.
+  rewrite stack_nwire_distribute_r.
+  rewrite stack_nwire_distribute_l.
+  repeat rewrite <- compose_assoc.
+  rewrite stack_assoc_back.
+  simpl_casts.
+  rewrite <- (stack_nwire_distribute_r (Z 1 (1 + 1) 0) (n_wire 1 ↕ Z 1 0 0 )).
+  rewrite <- grow_Z_bot_right.
+  rewrite compose_assoc.
+  rewrite <- stack_nwire_distribute_l.
+  rewrite <- X_appendix_rot_l.
+  rewrite Rplus_0_r.
+  rewrite Z_0_is_wire, X_0_is_wire.
+  rewrite <- wire_to_n_wire.
+  rewrite <- (stack_compose_distr — — — —).
+  cleanup_zx.
+  easy.
+Qed.
+
+Lemma cnot_is_cnot_r : _CNOT_ ∝ _CNOT_R.
+Proof.
+  intros.
+  remember (— ↕ X 1 2 0 ⟷ (Z 2 1 0 ↕ —)) as RHS.
+  rewrite (Z_wrap_under_bot_left 1 1).
+  rewrite (X_wrap_over_top_left 1 1).
+  simpl_casts.
+  rewrite wire_to_n_wire at 2 3 4 5.
+  rewrite stack_nwire_distribute_l.
+  rewrite stack_nwire_distribute_r.
+  repeat rewrite <- compose_assoc.
+  rewrite (compose_assoc _ (Z (1 + 1) 1 0 ↕ (n_wire _) ↕ _)).
+  rewrite stack_assoc.
+  simpl_casts.
+  rewrite n_wire_stack.
+  rewrite (nwire_stack_compose_botleft (Z (1 + 1) 1 0) (n_wire 1 ↕ X 1 2 0)).
+  rewrite <- (nwire_stack_compose_topleft (n_wire 1 ↕ X 1 2 0)).
+  rewrite <- compose_assoc.
+  rewrite stack_assoc_back.
+  simpl_casts.
+  rewrite n_wire_stack.
+  rewrite <- (stack_compose_distr ((n_wire 1) ↕ ⊂) (n_wire 3) (n_wire 1) (X 1 2 0)).
+  cleanup_zx.
+  rewrite <- nwire_stack_compose_topleft.
+  rewrite compose_assoc.
+  rewrite nwire_stack_compose_botleft.
+  rewrite <- (nwire_stack_compose_topleft (⊃ ↕ n_wire 1)).
+  rewrite <- compose_assoc.
+  rewrite (compose_assoc _ (n_wire 1 ↕ ⊂ ↕ n_wire 2) _).
+  simpl; cleanup_zx; simpl_casts.
+  rewrite 2 stack_assoc; simpl_casts.
+  rewrite <- stack_wire_distribute_l.
+  rewrite 2 stack_assoc_back; simpl_casts.
+  rewrite <- (stack_wire_distribute_r (⊂ ↕ —) (— ↕ ⊃)).
+  rewrite yank_r.
+  rewrite wire_to_n_wire.
+  rewrite 2 n_wire_stack.
+  cleanup_zx.
+  rewrite <- wire_to_n_wire.
+  subst.
+  easy.
 Qed.
